interface/Finite_set.fsti
@@ -1,0 +1,117 @@
+module Finite_set
+
+val t (a:eqtype) : Type0
+
+val empty (#a:eqtype) : t a
+val singleton (#a:eqtype) (x:a) : t a
+val mem (#a:eqtype) (x:a) (s:t a) : bool
+val equal (#a:eqtype) (s1:t a) (s2:t a) : Type0
+val union (#a:eqtype) (s1 s2:t a) : t a
+val intersection (#a:eqtype) (s1 s2:t a) : t a
+val complement : #a:eqtype -> (s:t a) -> t a
+val difference (#a:eqtype) (s1 s2:t a) : t a
+val filter (#a:eqtype) (s:t a) (p:a -> bool) : t a
+val remove (#a:eqtype) (s:t a) (x:a) : t a
+val cardinality (#a: eqtype) (s: t a) : GTot nat
+val choose (#a: eqtype) (s: t a{exists x. mem x s}) : GTot (x: a{mem x s})
+  
+val mem_empty (#a:eqtype) (x:a)
+  : Lemma (not (mem x empty))
+          [SMTPat (mem x empty)]
+
+val equal_intro (#a:eqtype) (s1 s2:t a)
+  : Lemma (requires (forall (x:a). mem x s1 == mem x s2))
+          (ensures equal s1 s2)
+          [SMTPat (equal s1 s2)]
+
+val equal_intro' (#a:eqtype) (s1 s2:t a)
+  : Lemma (ensures equal s1 s2 <==> s1 == s2)
+          [SMTPat (s1 == s2)]
+          
+val equal_elim (#a:eqtype) (s1 s2:t a)
+  : Lemma (requires equal s1 s2)
+          (ensures s1 == s2)
+          [SMTPat (equal s1 s2)]
+
+let equal_refl (#a:eqtype) (s1 s2:t a)
+  : Lemma (requires s1 == s2)
+          (ensures (forall (x:a). mem x s1 == mem x s2) /\ equal s1 s2)
+          [SMTPat (s1 == s2)] = ()
+          
+// no need to define it, it is already derivable
+let equal_refl1 (#a:eqtype) (s:t a)
+  : Lemma (equal s s) = ()
+
+let subset (#a:eqtype) (s1:t a) (s2:t a) =
+  (forall x. mem x s1 ==> mem x s2)
+
+val mem_subset (#a:eqtype) (s1:t a) (s2:t a)
+  : Lemma (requires (forall x. mem x s1 ==> mem x s2))
+          (ensures (subset s1 s2))
+          [SMTPat (subset s1 s2)]
+
+val subset_mem (#a:eqtype) (s1:t a) (s2:t a)
+  : Lemma (requires (subset s1 s2))
+          (ensures (forall x. mem x s1 ==> mem x s2))
+          [SMTPat (subset s1 s2)]
+   
+val mem_union (#a:eqtype) (s1 s2:t a) (x:a)
+  : Lemma (mem x (union s1 s2) <==> (mem x s1 || mem x s2))
+          [SMTPat (mem x (union s1 s2))]
+
+val mem_singleton: #a:eqtype -> x:a -> y:a -> Lemma
+   (requires True)
+   (ensures (mem y (singleton x) = (x=y)))
+   [SMTPat (mem y (singleton x))]
+   
+let add (#a:eqtype) (x:a) (s:t a) : t a =
+  union s (singleton x)
+
+val mem_intersection (#a:eqtype) (s1 s2:t a) (x:a)
+  : Lemma (mem x (intersection s1 s2) <==> (mem x s1 /\ mem x s2))
+          [SMTPat (mem x (intersection s1 s2))]
+
+val mem_complement (#a:eqtype) (s:t a) (x:a) 
+  : Lemma (mem x (complement s) = not (mem x s))
+   [SMTPat (mem x (complement s))]
+   
+val mem_difference (#a:eqtype) (s1 s2:t a) (x:a)
+  : Lemma (mem x (difference s1 s2) <==> (mem x s1 /\ ~ (mem x s2)))
+          [SMTPat (mem x (difference s1 s2))]
+   
+val mem_filter (#a:eqtype) (s:t a) (p:a -> bool) (x:a)
+  : Lemma (mem x (filter s p) <==> (mem x s /\ p x))
+          [SMTPat (mem x (filter s p))]
+
+val mem_remove_x (#a:eqtype) (s:t a) (x:a)
+  : Lemma (not (mem x (remove s x)))
+          [SMTPat (mem x (remove s x))]
+
+val mem_remove_y (#a:eqtype) (s:t a) (x:a) (y:a)
+  : Lemma (requires x =!= y)
+          (ensures mem y (remove s x) == mem y s)
+          [SMTPat (mem y (remove s x))]
+          
+val length_zero_fact (#a:eqtype) (s:t a)
+  : Lemma (ensures (cardinality s = 0 <==> s == empty)
+                   /\ (cardinality s <> 0 <==> (exists x. mem x s)))
+          [SMTPat (cardinality s)]
+
+val singleton_cardinality_fact (#a:eqtype) (r:a)
+  : Lemma (ensures cardinality (singleton r) = 1)
+    [SMTPat (cardinality (singleton r))]
+
+val intersection_cardinality_fact (#a:eqtype) (s1 s2:t a)
+  : Lemma (ensures cardinality (union s1 s2) + cardinality (intersection s1 s2) = cardinality s1 + cardinality s2)
+    [SMTPat (cardinality (intersection s1 s2))]
+    
+val difference_cardinality_fact (#a:eqtype) (s1 s2:t a)
+  : Lemma (ensures cardinality (difference s1 s2) + cardinality (difference s2 s1) + cardinality (intersection s1 s2) = cardinality (union s1 s2)
+    /\ cardinality (difference s1 s2) = cardinality s1 - cardinality (intersection s1 s2))
+    [SMTPat (cardinality (difference s1 s2))]
+
+val union_cardinality_fact (#a:eqtype) (s1 s2:t a)
+  : Lemma (ensures cardinality (difference s1 s2) + cardinality (difference s2 s1) + cardinality (intersection s1 s2) = cardinality (union s1 s2)
+    /\ cardinality (difference s1 s2) = cardinality s1 - cardinality (intersection s1 s2))
+    [SMTPat (cardinality (union s1 s2))]
+    
