interface/Ord_map.fst
@@ -1,0 +1,338 @@
+(*
+   Copyright 2008-2018 Microsoft Research
+
+   Licensed under the Apache License, Version 2.0 (the "License");
+   you may not use this file except in compliance with the License.
+   You may obtain a copy of the License at
+
+       http://www.apache.org/licenses/LICENSE-2.0
+
+   Unless required by applicable law or agreed to in writing, software
+   distributed under the License is distributed on an "AS IS" BASIS,
+   WITHOUT WARRANTIES OR CONDITIONS OF ANY KIND, either express or implied.
+   See the License for the specific language governing permissions and
+   limitations under the License.
+*)
+(**
+ * Implementation of partial maps with extensional equality
+ *)
+ 
+module Ord_map
+open FStar.FunctionalExtensionality
+module FLT = FStar.List.Tot
+module FSet = Finite_set //FStar.FiniteSet.Base
+open Finite_set //FStar.FiniteSet.Ambient
+module T = FStar.Tactics.V2
+
+(* The main "trick" in the representation of the type `t`
+ * is to use a domain-restricted function type `key ^-> value`
+ * from the FStar.FunctionalExtensionality library.
+ * These restricted function types enjoy extensional equality,
+ * which is necessary if Map.t is to also enjoy extensional equality.
+ *)
+
+type t (a: eqtype) (b: Type u#b) = (keys: FSet.t a) & (setfun_t a b keys)
+
+let domain (#a: eqtype) (#b: Type u#b) (m: t a b) : FSet.t a =
+  let (| keys, _ |) = m in 
+  keys
+  
+let elements (#a: eqtype) (#b: Type u#b) (m: t a b) : (setfun_t a b (domain m)) =
+  let (| _, f |) = m in
+  f
+
+let cardinality (#a: eqtype) (#b: Type u#b) (m: t a b) : GTot nat =
+  FSet.cardinality (domain m)
+
+(*let upd (#a: eqtype) (#b: Type u#b) (m: t a b) (k: a) (v: b) : t a b =
+  let keys' = FSet.insert k (domain m) in
+  let f' = on_domain a (fun key -> if key = k then Some v else (elements m) key) in
+  (| keys', f' |)*)
+
+let upd (#a: eqtype) (#b: Type u#b) (m: t a b) (k: a) (v: b) : t a b =
+  let keys' = FSet.union (FSet.singleton k) (domain m) in
+  let f' = on_domain a (fun key -> if key = k then Some v else (elements m) key) in
+  (| keys', f' |)
+  
+let emptymap (#a: eqtype) (#b: Type u#b) : (t a b) =
+  (| FSet.empty, on_domain a (fun key -> None) |)
+
+let subtract (#a: eqtype) (#b: Type u#b) (m: t a b) (s: FSet.t a) : t a b =
+  let keys' = FSet.difference (domain m) s in
+  let f' = on_domain a (fun key -> if FSet.mem key keys' then (elements m) key else None) in
+  (| keys', f' |)
+
+let map_val (#a: eqtype) (#b: Type u#b) (#c: Type u#c)
+            (f: b -> c)
+            (m: t a b)
+            : t a c =
+  let keys = domain m in
+  let new_setfun = on_domain a (fun (key: a) -> 
+    match (elements m) key with
+    | Some v -> Some (f v)
+    | None -> None)
+  in
+  (|keys, new_setfun|)
+
+let iter_upd (#a: eqtype) (#b: Type u#b) (#c: Type u#c)
+            (f: a -> b -> c)
+            (m: t a b)
+            : t a c =
+  let keys = domain m in
+  let new_setfun = on_domain a (fun (key: a) -> 
+    match (elements m) key with
+    | Some v -> Some (f key v)
+    | None -> None)
+  in
+  (|keys, new_setfun|)
+ 
+let const_on (#a: eqtype) (#b: Type u#b)
+             (keys: FSet.t a)
+             (value: b)
+             : t a b =
+  let setfun = on_domain a (fun (key: a) ->
+    if FSet.mem key keys then Some value else None)
+  in
+  (|keys, setfun|)
+  
+let values (#a: eqtype) (#b: Type u#b) (m: t a b) : GTot (b -> prop) =
+  fun value -> exists key. ((elements m) key == Some value)
+
+let items (#a: eqtype) (#b: Type u#b) (m: t a b) : GTot ((a * b) -> prop) =
+  fun item -> ((elements m) (fst item) == Some (snd item))
+
+let equal (#a: eqtype) (#b: Type u#b) (m1: t a b) (m2: t a b) : prop =
+  feq (elements m1) (elements m2) /\ True //a bit ugly, a prop coercion
+
+let choose (#a: eqtype) (#b: Type u#b) (m: t a b{exists key. mem key m}) : GTot (key: a{mem key m}) =
+  FSet.choose (domain m)
+
+let cardinality_zero_iff_empty_fact' m = 
+  introduce forall (a: eqtype) (b:Type u#b) (m: t a b). cardinality m = 0 <==> m == emptymap
+  with (
+    introduce cardinality m = 0 ==> m == emptymap
+    with _. assert (feq (elements m) (elements emptymap))
+  )
+  
+let empty_or_domain_occupied_fact' m = 
+  introduce forall (a: eqtype) (b:Type u#b) (m: t a b). m == emptymap \/ (exists k. mem k m)
+    with (  
+    if FSet.cardinality (domain m) = 0 then
+      introduce m == emptymap \/ (exists k. mem k m)
+      with Left (
+        assert (cardinality m = 0);
+        cardinality_zero_iff_empty_fact' m
+      )
+    else
+      introduce m == emptymap \/ (exists k. mem k m)
+      with Right ()
+    )
+
+let empty_or_values_occupied_fact' m = 
+  introduce forall (a: eqtype) (b:Type u#b) (m: t a b). m == emptymap \/ (exists v. (values m) v)
+  with
+    if FSet.cardinality (domain m) = 0 then
+      introduce m == emptymap \/ (exists v. (values m) v)
+      with Left (
+        assert (cardinality m = 0);
+        cardinality_zero_iff_empty_fact' m
+      )
+    else
+      introduce m == emptymap \/ (exists v. (values m) v)
+      with Right (
+        let k = choose m in
+        let v = Some?.v ((elements m) k) in
+        assert ((values m) v)
+      )
+
+let empty_or_items_occupied_fact' m =
+  introduce forall (a: eqtype) (b: Type u#b) (m: t a b). m == emptymap \/ (exists item. (items m) item)
+  with
+    if FSet.cardinality (domain m) = 0 then
+      introduce m == emptymap \/ (exists v. (values m) v)
+      with Left (
+        assert (cardinality m = 0);
+        cardinality_zero_iff_empty_fact' m
+      )
+    else
+      introduce m == emptymap \/ (exists item. (items m) item)
+      with Right (
+        let k = choose m in
+        let v = Some?.v ((elements m) k) in
+        assert ((items m) (k, v))
+      )
+
+let map_cardinality_matches_domain_fact' m = ()
+let values_contains_fact' m v = ()
+let items_contains_fact' m item = ()
+let empty_domain_empty_fact' u = ()
+
+#set-options "--z3rlimit 300 --ifuel 3"
+let upd_elements_fact' m k k' v = ()
+
+let const_on_elements_fact' s v = ()
+let cons_on_member_cardinality_fact' s v = ()
+
+let upd_member_cardinality_fact' m k v = ()
+
+let upd_nonmember_cardinality_fact' m k v = ()
+
+let iter_upd_domain_fact' f m = ()
+
+let iter_upd_element_fact' f m k = ()
+
+let subtract_domain_fact' m s = ()
+let subtract_element_fact' m s k = ()
+let map_equal_fact' m1 m2 = ()
+let map_extensionality_fact' m1 m2 = 
+  introduce forall (a: eqtype) (b:Type u#b) (m1: t a b) (m2: t a b). equal m1 m2 ==> m1 == m2
+  with (
+    introduce equal m1 m2 ==> m1 == m2
+    with _. (
+      assert (FSet.equal (domain m1) (domain m2));
+      assert (feq (elements m1) (elements m2))
+    )
+  )
+
+(*let cardinality_zero_iff_empty_lemma ()
+: Lemma (cardinality_zero_iff_empty_fact u#b) =
+  introduce forall (a: eqtype) (b:Type u#b) (m: t a b). cardinality m = 0 <==> m == emptymap
+  with (
+    introduce cardinality m = 0 ==> m == emptymap
+    with _. assert (feq (elements m) (elements emptymap))
+  )
+
+let empty_or_domain_occupied_lemma ()
+  : Lemma (empty_or_domain_occupied_fact u#b)
+  = introduce forall (a: eqtype) (b:Type u#b) (m: t a b). m == emptymap \/ (exists k. mem k m)
+    with (  
+    if FSet.cardinality (domain m) = 0 then
+      introduce m == emptymap \/ (exists k. mem k m)
+      with Left (
+        assert (cardinality m = 0);
+        cardinality_zero_iff_empty_lemma ()
+      )
+    else
+      introduce m == emptymap \/ (exists k. mem k m)
+      with Right ()
+    )
+
+let empty_or_values_occupied_lemma ()
+: Lemma (empty_or_values_occupied_fact u#b) =
+  introduce forall (a: eqtype) (b:Type u#b) (m: t a b). m == emptymap \/ (exists v. (values m) v)
+  with
+    if FSet.cardinality (domain m) = 0 then
+      introduce m == emptymap \/ (exists v. (values m) v)
+      with Left (
+        assert (cardinality m = 0);
+        cardinality_zero_iff_empty_lemma u#b ()
+      )
+    else
+      introduce m == emptymap \/ (exists v. (values m) v)
+      with Right (
+        let k = choose m in
+        let v = Some?.v ((elements m) k) in
+        assert ((values m) v)
+      )
+
+let empty_or_items_occupied_lemma ()
+: Lemma (empty_or_items_occupied_fact u#b) =
+  introduce forall (a: eqtype) (b: Type u#b) (m: t a b). m == emptymap \/ (exists item. (items m) item)
+  with
+    if FSet.cardinality (domain m) = 0 then
+      introduce m == emptymap \/ (exists v. (values m) v)
+      with Left (
+        assert (cardinality m = 0);
+        cardinality_zero_iff_empty_lemma u#b ()
+      )
+    else
+      introduce m == emptymap \/ (exists item. (items m) item)
+      with Right (
+        let k = choose m in
+        let v = Some?.v ((elements m) k) in
+        assert ((items m) (k, v))
+      )
+
+let map_cardinality_matches_domain_lemma ()
+: Lemma (map_cardinality_matches_domain_fact u#b) =
+  ()
+
+let values_contains_lemma ()
+: Lemma (values_contains_fact u#b) =
+  ()
+
+let items_contains_lemma ()
+: Lemma (items_contains_fact u#b) =
+  ()
+
+let empty_domain_empty_lemma ()
+: Lemma (empty_domain_empty_fact u#b) =
+  ()
+
+let upd_elements_lemma ()
+: Lemma (upd_elements_fact u#b) =
+  ()
+
+let upd_member_cardinality_lemma ()
+: Lemma (upd_member_cardinality_fact u#b) =
+  ()
+
+let upd_nonmember_cardinality_lemma ()
+: Lemma (upd_nonmember_cardinality_fact u#b) =
+  ()
+
+let subtract_domain_lemma ()
+: Lemma (subtract_domain_fact u#b) =
+  ()
+
+let subtract_element_lemma ()
+: Lemma (subtract_element_fact u#b) =
+  ()
+
+
+let map_equal_lemma ()
+: Lemma (map_equal_fact u#b) //Surprising; needed to split this goal into two
+= assert (map_equal_fact u#b)
+    by (T.norm [delta_only [`%map_equal_fact]];
+        let _ = T.forall_intro () in
+        let _ = T.forall_intro () in
+        let _ = T.forall_intro () in         
+        let _ = T.forall_intro () in                 
+        T.split ();
+        T.smt();
+        T.smt())
+
+
+let map_extensionality_lemma ()
+: Lemma (map_extensionality_fact u#b) =
+  introduce forall (a: eqtype) (b:Type u#b) (m1: t a b) (m2: t a b). equal m1 m2 ==> m1 == m2
+  with (
+    introduce equal m1 m2 ==> m1 == m2
+    with _. (
+      assert (FSet.equal (domain m1) (domain m2));
+      assert (feq (elements m1) (elements m2))
+    )
+  )
+
+let lemma_equal_intro m1 m2 = ()
+let lemma_equal_elim m1 m2 = admit()
+let lemma_equal_intro' m1 m2 = admit()
+
+let all_finite_map_facts_lemma (_:unit)
+  : Lemma (all_finite_map_facts u#b)
+  = cardinality_zero_iff_empty_lemma u#b ();
+    empty_or_domain_occupied_lemma u#b ();
+    empty_or_values_occupied_lemma u#b ();
+    empty_or_items_occupied_lemma u#b ();
+    map_cardinality_matches_domain_lemma u#b ();
+    values_contains_lemma u#b ();
+    items_contains_lemma u#b ();
+    empty_domain_empty_lemma u#b ();
+    upd_elements_lemma u#b ();
+    upd_member_cardinality_lemma u#b ();
+    upd_nonmember_cardinality_lemma u#b ();
+    subtract_domain_lemma u#b ();
+    subtract_element_lemma u#b ();
+    map_equal_lemma u#b ();
+    map_extensionality_lemma u#b ()
+*)
