interface/Ord_map.fsti
@@ -1,0 +1,297 @@
+(*
+   Copyright 2008-2018 Microsoft Research
+
+   Licensed under the Apache License, Version 2.0 (the "License");
+   you may not use this file except in compliance with the License.
+   You may obtain a copy of the License at
+
+       http://www.apache.org/licenses/LICENSE-2.0
+
+   Unless required by applicable law or agreed to in writing, software
+   distributed under the License is distributed on an "AS IS" BASIS,
+   WITHOUT WARRANTIES OR CONDITIONS OF ANY KIND, either express or implied.
+   See the License for the specific language governing permissions and
+   limitations under the License.
+*)
+
+(**
+
+ @summary FStar.Map provides a polymorphic, partial map from keys to
+   values, where keys support decidable equality.
+
+ `m:Map.t key value` is a partial map from `key` to `value`
+
+  A distinctive feature of the library is in its model of partiality.
+
+  A map can be seen as a pair of:
+    1. a total map `key -> Tot value`
+    2. a set of keys that record the domain of the map
+
+*)
+module Ord_map
+
+//module S = Set_extended
+open FStar.FunctionalExtensionality
+module FSet = Finite_set //FStar.FiniteSet.Base
+
+type setfun_t (a: eqtype)
+              (b: Type u#b)
+              (s: FSet.t a) =
+   f: (a ^-> option b){forall (key: a). FSet.mem key s == Some? (f key)}
+   
+(* Map.t key value: The main type provided by this module *)
+val t (key:eqtype) ([@@@strictly_positive] value:Type u#a)
+  : Type u#a
+
+(* domain m : The set of keys on which this partial map is defined *)
+val domain: #key:eqtype -> #value:Type -> t key value -> Tot (FSet.t key)
+
+val elements (#a: eqtype) (#b: Type u#b) (m: t a b)
+  : setfun_t a b (domain m)
+  
+let contains (#a: eqtype) (#b: Type u#b) (m: t a b) (key: a) =
+  FSet.mem key (domain m)
+  
+let sel (#a: eqtype) (#b: Type u#b) (key: a) (m: t a b{contains m key}) : b =
+  Some?.v ((elements m) key)
+
+val cardinality: #key:eqtype -> #value:Type -> t key value -> GTot nat
+  
+val upd (#a: eqtype) (#b: Type u#b) (m: t a b) (k: a) (v: b) : t a b
+  
+val emptymap (#a: eqtype) (#b: Type u#b) : t a b
+
+val subtract (#a: eqtype) (#b: Type u#b) (m: t a b) (s: FSet.t a) : t a b
+
+let remove (#a: eqtype) (#b: Type u#b) (key: a) (m: t a b) : t a b =
+  subtract m (FSet.singleton key)
+
+(*let upd (#a: eqtype) (#b: Type u#b) (m: t a b) (k: a) (v: b) =
+  let r = remove k m in
+  insert r k v*)
+
+val map_val: #key:eqtype -> #val1:Type u#b -> #val2:Type u#c -> f:(val1 -> val2) -> t key val1 -> Tot (t key val2)
+
+val iter_upd: #key:eqtype -> #val1:Type u#b -> #val2:Type u#c -> f:(key -> val1 -> val2) -> t key val1 -> Tot (t key val2)
+
+val const_on: #key:eqtype -> #val1:Type u#b -> k:(FSet.t key) -> val1 -> Tot (t key val1)
+
+val values (#a: eqtype) (#b: Type u#b) (m: t a b)
+  : GTot (b -> prop)
+
+val items (#a: eqtype) (#b: Type u#b) (m: t a b)
+  : GTot ((a * b) -> prop)
+
+val equal (#a: eqtype) (#b: Type u#b) (m1: t a b) (m2: t a b)
+  : prop
+
+let mem (#a: eqtype) (#b: Type u#b) (key: a) (m: t a b) =
+  FSet.mem key (domain m)
+
+val choose (#a: eqtype) (#b: Type u#b) (m: t a b{exists key. mem key m})
+  : GTot (key: a{mem key m})
+
+val cardinality_zero_iff_empty_fact' (#k: eqtype) (#v: Type u#b) (m: t k v)
+  : Lemma (ensures cardinality m = 0 <==> m == emptymap)
+          [SMTPat (cardinality m)]
+
+(*let cardinality_zero_iff_empty_fact =
+  forall (k: eqtype) (v:Type u#b) (m: t k v).{:pattern cardinality m}
+    cardinality m = 0 <==> m == emptymap*)
+
+val empty_or_domain_occupied_fact' (#k: eqtype) (#v: Type u#b) (m: t k v)
+  : Lemma (ensures m == emptymap \/ (exists k. mem k m))
+          [SMTPat (domain m)]
+          
+(*let empty_or_domain_occupied_fact =
+  forall (a: eqtype) (b: Type u#b) (m: t a b).{:pattern domain m}
+    m == emptymap \/ (exists k.{:pattern mem k m} mem k m)*)
+
+val empty_or_values_occupied_fact' (#k: eqtype) (#v: Type u#b) (m: t k v)
+  : Lemma (ensures m == emptymap \/ (exists v. (values m) v))
+          [SMTPat (values m v)]
+  
+(*let empty_or_values_occupied_fact =
+  forall (a: eqtype) (b: Type u#b) (m: t a b).{:pattern values m}
+    m == emptymap \/ (exists v. {:pattern values m v } (values m) v)*)
+
+val empty_or_items_occupied_fact' (#k: eqtype) (#v: Type u#b) (m: t k v)
+  : Lemma (ensures m == emptymap \/ (exists item. (items m) item))
+          [SMTPat (exists item. items m item)]
+   
+(*let empty_or_items_occupied_fact =
+  forall (a: eqtype) (b:Type u#b) (m: t a b).{:pattern items m}
+    m == emptymap \/ (exists item. {:pattern items m item } (items m) item)*)
+
+val map_cardinality_matches_domain_fact' (#k: eqtype) (#v: Type u#b) (m: t k v)
+  : Lemma (ensures FSet.cardinality (domain m) = cardinality m)
+          [SMTPat (FSet.cardinality (domain m))]
+
+(*let map_cardinality_matches_domain_fact =
+  forall (a: eqtype) (b: Type u#b) (m: t a b).{:pattern FSet.cardinality (domain m)}
+    FSet.cardinality (domain m) = cardinality m*)
+
+val values_contains_fact' (#a: eqtype) (#b: Type u#b) (m: t a b) (v:b) 
+  : Lemma (ensures (values m) v <==>
+       (exists (u: a).FSet.mem u (domain m) /\ (elements m) u == Some v))
+       [SMTPat ((values m) v)]
+  
+(*let values_contains_fact =
+  forall (a: eqtype) (b: Type u#b) (m: t a b) (v: b).{:pattern (values m) v}
+    (values m) v <==>
+       (exists (u: a).{:pattern FSet.mem u (domain m) \/ ((elements m) u)}
+          FSet.mem u (domain m) /\ (elements m) u == Some v)*)
+
+val items_contains_fact' (#a: eqtype) (#b: Type u#b) (m: t a b) (item: a * b)
+  : Lemma (ensures (items m) item <==>
+        FSet.mem (fst item) (domain m)
+      /\ (elements m) (fst item) == Some (snd item))
+        [SMTPat ((items m) item)]
+
+(*let items_contains_fact =
+  forall (a: eqtype) (b: Type u#b) (m: t a b) (item: a * b).{:pattern (items m) item}
+    (items m) item <==>
+        FSet.mem (fst item) (domain m)
+      /\ (elements m) (fst item) == Some (snd item)*)
+
+val empty_domain_empty_fact' (#a: eqtype) (#b: Type u#b) (u:a)
+  : Lemma (ensures not (FSet.mem u (domain (emptymap #a #b))))
+          [SMTPat (FSet.mem u (domain (emptymap #a #b)))]
+
+(*let empty_domain_empty_fact =
+  forall (a: eqtype) (b: Type u#b) (u: a).{:pattern FSet.mem u (domain (emptymap #a #b))}
+    not (FSet.mem u (domain (emptymap #a #b)))*)
+
+val upd_elements_fact' (#a: eqtype) (#b: Type u#b) (m: t a b) (key:a) (key':a) (value:b)
+  : Lemma (ensures (key' = key ==>   FSet.mem key' (domain (upd m key value))
+                     /\ (elements (upd m key value)) key' == Some value)
+    /\ (key' <> key ==>   FSet.mem key' (domain (upd m key value)) = FSet.mem key' (domain m)
+                     /\ (elements (upd m key value)) key' == (elements m) key'))
+                     [SMTPat (upd m key value)]
+
+val const_on_elements_fact' (#a: eqtype) (#b: Type u#b) (s: FSet.t a) (value:b)
+  : Lemma (ensures (forall k. FSet.mem k s <==> (FSet.mem k (domain (const_on s value)))) /\
+                   (forall k. FSet.mem k s ==> (elements (const_on s value)) k == Some value))
+          [SMTPat (const_on s value)]
+  
+  (*(key' = key ==>   FSet.mem key' (domain (upd m key value))
+                     /\ (elements (upd m key value)) key' == Some value)
+    /\ (key' <> key ==>   FSet.mem key' (domain (upd m key value)) = FSet.mem key' (domain m)
+                     /\ (elements (upd m key value)) key' == (elements m) key'))
+                     [SMTPat (upd m key value)]*)
+
+val cons_on_member_cardinality_fact' (#a: eqtype) (#b: Type u#b) (s: FSet.t a) (value:b)
+  : Lemma (ensures (forall k. FSet.mem k (domain (const_on s value)) ==> cardinality (const_on s value) = FSet.cardinality s))
+    [SMTPat (cardinality (const_on s value))]
+
+(*let upd_elements_fact =
+  forall (a: eqtype) (b: Type u#b) (m: t a b) (key: a) (key': a) (value: b).
+    {:pattern FSet.mem key' (domain (upd m key value)) \/ ((elements (upd m key value)) key')}
+      (key' = key ==>   FSet.mem key' (domain (upd m key value))
+                     /\ (elements (upd m key value)) key' == Some value)
+    /\ (key' <> key ==>   FSet.mem key' (domain (upd m key value)) = FSet.mem key' (domain m)
+                     /\ (elements (upd m key value)) key' == (elements m) key')*)
+
+val upd_member_cardinality_fact' (#a: eqtype) (#b: Type u#b) (m: t a b) (key:a) (value:b)
+  : Lemma (ensures FSet.mem key (domain m) ==> cardinality (upd m key value) = cardinality m)
+    [SMTPat (cardinality (upd m key value))]
+
+(*let upd_member_cardinality_fact =
+  forall (a: eqtype) (b: Type u#b) (m: t a b) (key: a) (value: b).{:pattern cardinality (upd m key value)}
+    FSet.mem key (domain m) ==> cardinality (upd m key value) = cardinality m*)
+
+val upd_nonmember_cardinality_fact' (#a: eqtype) (#b: Type u#b) (m: t a b) (key: a) (value: b)
+  : Lemma (not (FSet.mem key (domain m)) ==> cardinality (upd m key value) = cardinality m + 1)
+    [SMTPat (cardinality (upd m key value))]
+  
+(*let upd_nonmember_cardinality_fact =
+  forall (a: eqtype) (b: Type u#b) (m: t a b) (key: a) (value: b).{:pattern cardinality (upd m key value)}
+    not (FSet.mem key (domain m)) ==> cardinality (upd m key value) = cardinality m + 1*)
+
+val iter_upd_domain_fact' (#a: eqtype) (#b: Type u#b) (#c: Type u#c) (f:a -> b -> c) (m: t a b) 
+  : Lemma (ensures domain (iter_upd f m) == domain m)
+          [SMTPat (domain (iter_upd f m))]
+
+val iter_upd_element_fact' (#a: eqtype) (#b: Type u#b) (#c: Type u#c) (f:a -> b -> c) (m: t a b) (key:a)
+  : Lemma (ensures FSet.mem key (domain (iter_upd f m)) ==> FSet.mem key (domain m) /\ 
+                   (if Some? ((elements m) key) then 
+                     (let Some v = (elements m) key in
+                       (elements (iter_upd f m)) key == Some (f key v)) //(f key v))
+                    else true))
+    [SMTPat ((elements (iter_upd f m)) key)]
+
+val subtract_domain_fact' (#a: eqtype) (#b: Type u#b) (m: t a b) (s:FSet.t a)
+  : Lemma (ensures domain (subtract m s) == FSet.difference (domain m) s)
+          [SMTPat (domain (subtract m s))]
+
+(*let subtract_domain_fact =
+  forall (a: eqtype) (b: Type u#b) (m: t a b) (s: FSet.set a).{:pattern domain (subtract m s)}
+    domain (subtract m s) == FSet.difference (domain m) s*)
+
+val subtract_element_fact' (#a: eqtype) (#b: Type u#b) (m: t a b) (s:FSet.t a) (key:a) 
+  : Lemma (ensures FSet.mem key (domain (subtract m s)) ==> FSet.mem key (domain m) /\ (elements (subtract m s)) key == (elements m) key)
+    [SMTPat ((elements (subtract m s)) key)]
+
+(*let subtract_element_fact =
+  forall (a: eqtype) (b: Type u#b) (m: t a b) (s: FSet.set a) (key: a).{:pattern (elements (subtract m s)) key}
+    FSet.mem key (domain (subtract m s)) ==> FSet.mem key (domain m) /\ (elements (subtract m s)) key == (elements m) key*)
+
+val map_equal_fact' (#a: eqtype) (#b: Type u#b) (m1 m2: t a b) 
+  : Lemma (ensures equal m1 m2 <==>   (forall key. FSet.mem key (domain m1) = FSet.mem key (domain m2))
+                   /\ (forall key. FSet.mem key (domain m1) ==> (elements m1) key == (elements m2) key))
+    [SMTPat (equal m1 m2)]
+
+(*let map_equal_fact =
+  forall (a: eqtype) (b: Type u#b) (m1: t a b) (m2: t a b).{:pattern equal m1 m2}
+    equal m1 m2 <==>   (forall key. FSet.mem key (domain m1) = FSet.mem key (domain m2))
+                   /\ (forall key. FSet.mem key (domain m1) ==> (elements m1) key == (elements m2) key)*)
+
+val map_extensionality_fact' (#a: eqtype) (#b: Type u#b) (m1 m2: t a b) 
+  : Lemma (ensures equal m1 m2 ==> m1 == m2)
+    [SMTPat (equal m1 m2)]
+
+(*let map_extensionality_fact =
+  forall (a: eqtype) (b: Type u#b) (m1: t a b) (m2: t a b).{:pattern equal m1 m2}
+    equal m1 m2 ==> m1 == m2*)
+
+(*val lemma_equal_intro: #key:eqtype -> #value:Type -> m1:t key value -> m2:t key value ->
+                       Lemma (requires (forall k. contains m1 k /\ contains m2 k /\ 
+                                             sel k m1 == sel k m2))
+                             (ensures (equal m1 m2))
+                             [SMTPat (equal m1 m2)]
+
+val lemma_equal_elim: #key:eqtype -> #value:Type -> m1:t key value -> m2:t key value ->
+                      Lemma (ensures (equal m1 m2 <==> m1 == m2))
+                            [SMTPat (equal m1 m2)]
+
+val lemma_equal_intro': #key:eqtype -> #value:Type -> m1:t key value -> m2:t key value ->
+                       Lemma (requires (equal m1 m2))
+                             (ensures (forall k. contains m1 k /\ contains m2 k /\ 
+                                             sel k m1 == sel k m2))
+                             [SMTPat (equal m1 m2)]*)
+
+(*let equal_refl (#key:eqtype) (#value:Type) (m1:t key value) (m2:t key value) :
+    Lemma (requires m1 == m2)
+          (ensures (forall k. (contains m1 k = contains m2 k) /\ sel k m1 == sel k m2))
+          [SMTPat (m1 == m2)] = ()*)
+          
+(*let all_finite_map_facts =
+    cardinality_zero_iff_empty_fact u#b
+  /\ empty_or_domain_occupied_fact u#b
+  /\ empty_or_values_occupied_fact u#b
+  /\ empty_or_items_occupied_fact u#b
+  /\ map_cardinality_matches_domain_fact u#b
+  /\ values_contains_fact u#b
+  /\ items_contains_fact u#b
+  /\ empty_domain_empty_fact u#b
+  /\ upd_elements_fact u#b
+  /\ upd_member_cardinality_fact u#b
+  /\ upd_nonmember_cardinality_fact u#b
+  /\ subtract_domain_fact u#b
+  /\ subtract_element_fact u#b
+  /\ map_equal_fact u#b
+  /\ map_extensionality_fact u#b
+  
+val all_finite_map_facts_lemma (_:unit)
+  : Lemma (all_finite_map_facts u#b)*)
+
